docs/03-formal-verification/easycrypt/games/GameMSHopCompositionParameterized.ec
@@ -5,10 +5,12 @@ require import SourceTypes.
 require import SourceDistributions SourceTheorem MS.
 require import MSProbabilitySurface.
 require import GameAdvantage.
+require import GameAdvantageParameterized.
 require import GameViews.
 require import GameMSHopTypes.
 require import GameMSHopTransitions.
 require import GameMSHopTypesParameterized.
+require import SourceHashBindingSemanticSlotMassParameterized.
 require ParameterizedBudgetParameters.
 
 (*---*) import RealOrder.
@@ -99,9 +101,9 @@ qed.
 lemma A_MS1_hash_binding_parameterized_staged_composition_bound :
   forall (x : qssm_public_input) (s : seed) (xms : ms_public_input)
          (D : distinguisher),
-    game_pr_ms_public_endpoint_core x s xms MSPublicEndpointAfterBinding D -
+    game_pr_ms_public_endpoint_core_parameterized x s xms MSPublicEndpointAfterBinding D -
     ms_view_distinguish_pr (d_ms_after_binding_observable_v2 x s xms) D <=
-  MS.epsilon_ms_hash_binding_semantic.
+  ms_hash_binding_local_public_divergence_upper_mass_parameterized.
 proof.
 move=> x s xms D.
 exact (A_MS1_hash_binding_parameterized_stage_bound x s xms D).
@@ -121,8 +123,8 @@ qed.
 lemma A_MS_public_endpoint_parameterized_staged_composition_bound :
   forall (x : qssm_public_input) (xms : ms_public_input) (s : seed)
          (D : distinguisher),
-    Adv_ms_public_endpoint x s xms D <=
-  MS.epsilon_ms_hash_binding_semantic +
+    Adv_ms_public_endpoint_parameterized x s xms D <=
+  ms_hash_binding_local_public_divergence_upper_mass_parameterized +
       ParameterizedBudgetParameters.epsilon_ms_rom_programmability_parameterized.
 proof.
 move=> x xms s D.
